Added LE instruction and proofs.

src/coq/App/Instruction.v
@@ -18,7 +18,8 @@ Inductive Instruction : Type :=
     | XOR : Instruction
     | EQL : Instruction
     | LT : Instruction
-    | GT : Instruction.
+    | GT : Instruction
+    | LE : Instruction.
 
 (* The time to execute a NOP instruction. *)
 Definition NOP_DELAY : nat := 1.
@@ -58,5 +59,8 @@ Definition LT_DELAY : nat := 2.
 
 (* The time to execute a GT instruction. *)
 Definition GT_DELAY : nat := 2.
+
+(* The time to execute a LE instruction. *)
+Definition LE_DELAY : nat := 2.
 
 End Instruction.
